compiler/bootstrap/translation/to_bviProgScript.sml
@@ -7,6 +7,7 @@ val _ = new_theory "to_bviProg";
 val _ = translation_extends "to_bvlProg";
 
 val _ = ml_translatorLib.ml_prog_update (ml_progLib.open_module "to_bviProg");
+val _ = ml_translatorLib.use_string_type true;
 
 (* ------------------------------------------------------------------------- *)
 (* Setup                                                                     *)
